theories/Confluence.v
@@ -3,7 +3,7 @@
 From Stdlib Require Import Utf8 List Arith Bool Lia.
 From TypedConfluence.autosubst
 Require Import core unscoped AST SubstNotations RAsimpl AST_rasimpl.
-From TypedConfluence Require Import Util BasicAST Weakenings Contexts Typing. (*  Env Inst. *)
+From TypedConfluence Require Import Util BasicAST Weakenings Contexts Typing BasicMetaTheory. (*  Env Inst. *)
 From Stdlib Require Import Setoid Morphisms Relation_Definitions.
 
 Reserved Notation "Γ ⊢< l > t ⟹ u : T" (at level 50, l, t, u, T at next level).
@@ -182,8 +182,119 @@ Proof.
   split; apply ortho_irrel; auto.
 Qed. 
 
-(* to prove the diamond property, an induction on t will not work, because in rule eta the subject of the premises are not subterms of t. 
-  we instead need a measure stable under weakenings, like the size of t. *)
+
+(* Inversion principles for ⟹ *)
+
+Lemma ortho_var_inv Γ i x t A :
+  Γ ⊢< ty i > var x ⟹ t : A →
+  ∃ B,
+    t = var x  ∧
+    ⊢ Γ ∧
+    nth_error Γ x = Some (ty i, B) ∧
+    Γ ⊢< Ax (ty i) > (plus (S x)) ⋅ B ≡ A : Sort (ty i).
+Proof.
+Admitted.
+
+Lemma ortho_sort_inv Γ l l' t A :
+  Γ ⊢< l' > Sort l ⟹ t : A →
+  ⊢ Γ ∧
+  t = Sort l  ∧ l' = Ax (Ax l)  ∧
+  Γ ⊢< Ax (Ax (Ax l)) > Sort (Ax l) ≡ A : Sort (Ax l).
+Proof.
+Admitted.
+
+Lemma ortho_pi_inv Γ l1 l2 l' t' A B T :
+  Γ ⊢< l' > Pi l1 l2 A B ⟹ t' : T →
+  exists A' B',
+    t' = Pi l1 l2 A' B'  ∧
+    l' =  Ax (Ru l1 l2) ∧
+    Γ ⊢< Ax l1 > A ⟹ A' : Sort l1 ∧
+    Γ ,, (l1 , A) ⊢< Ax l2 > B ⟹ B' : Sort l2 ∧
+    Γ ⊢< Ax (Ax (Ru l1 l2)) > Sort (Ru l1 l2) ≡ T : Sort (Ax (Ru l1 l2)).
+Proof.
+Admitted.
+
+Lemma ortho_lam_inv Γ i l1 l2 A1 B1 t u T :
+  Γ ⊢< ty i > lam l1 l2 A1 B1 t ⟹ u : T →
+  ty i = Ru l1 l2 ∧ 
+  Γ ⊢< Ax (Ru l1 l2) > Pi l1 l2 A1 B1 ≡ T : Sort (Ru l1 l2)  ∧
+ (( (* a congruence rule *)
+    exists A1' B1' t',
+      u = lam l1 l2 A1' B1' t' ∧
+      Γ ⊢< Ax l1 > A1 ≡ A1' : Sort l1 ∧
+      Γ ,, (l1 , A1) ⊢< Ax l2 > B1 ≡ B1' : Sort l2 ∧
+      Γ ,, (l1 , A1) ⊢< l2 > t ⟹ t' : B1
+  ) \/ ( (* an application of eta*)
+    exists A2 B2 v v',
+
+      let v_wk := wk_tm (_wk_step _wk_id) v in 
+      let A2_wk := wk_tm (_wk_step _wk_id) A2 in 
+      let B2_wk := wk_tm (_wk_up (_wk_step _wk_id)) B2 in
+      t = app l1 l2 A2_wk B2_wk v_wk (var 0)  ∧
+      
+      Γ ⊢< Ax l1 > A1 ≡ A2 : Sort l1  ∧
+      Γ ,, (l1 , A1) ⊢< Ax l2 > B1 ≡ B2 : Sort l2  ∧
+      Γ ⊢< Ru l1 l2 > v ⟹ v' : Pi l1 l2 A1 B1  ∧
+      u = v'
+  )).
+Admitted.
+
+Lemma ortho_app_inv Γ i l1 l2 A1 B1 t u w T :
+  Γ ⊢< ty i > app l1 l2 A1 B1 t u ⟹ w : T →
+  ty i = l2 ∧ 
+  Γ ⊢< Ax l2 > B1 <[ u .. ] ≡ T : Sort l2  ∧
+  ((
+    (* by app cong *)
+    exists A1' B1' t' u',
+      w = app l1 l2 A1' B1' t' u' ∧
+      Γ ⊢< Ax l1 > A1 ≡ A1' : Sort l1 ∧
+      Γ ,, (l1 , A1) ⊢< Ax l2 > B1 ≡ B1' : Sort l2 ∧
+      Γ ⊢< Ru l1 l2 > t ⟹ t' : Pi l1 l2 A1 B1  ∧
+      Γ ⊢< l1 > u ⟹ u' : A1
+  ) \/ (
+    (* by beta *)
+    exists A2 B2 v v' u',
+      t = lam l1 l2 A2 B2 v  ∧
+      Γ ⊢< Ax l1 > A1 ≡ A2 : Sort l1 ∧
+      Γ ,, (l1 , A1) ⊢< Ax l2 > B1 ≡ B2 : Sort l2 ∧
+      Γ ,, (l1 , A1) ⊢< l2 > v ⟹ v' : B1  ∧
+      Γ ⊢< l1 > u ⟹ u' : A1  ∧
+      w = v' <[ u' .. ]
+  )).
+Admitted.
+
+
+(* TODO finish *)
+
+Ltac ttinv h :=
+  lazymatch type of h with
+  _ ⊢< _ > ?t ⟹ _ : _ =>
+    lazymatch t with
+    | var _ => eapply ortho_var_inv in h
+    | Sort _ => eapply ortho_sort_inv in h
+    | Pi _ _ _ _ => eapply ortho_pi_inv in h
+    | lam _ _ _ _ _ => eapply ortho_lam_inv in h as h'
+    | app _ _ _ _ _ _ => eapply ortho_app_inv in h as h'
+    | _ => h
+    end
+  end.
+
+
+
+(* allows us to close the diamond with different types in the two ends *)
+Lemma ortho_diamond_helper Γ l t t' t'' A :
+  Γ ⊢< l > t ⟹ t' : A -> 
+  Γ ⊢< l > t ⟹ t'' : A -> 
+    (exists B C l' l'' t''', (Γ ⊢< l' > t' ⟹ t''' : B) /\ (Γ ⊢< l'' > t'' ⟹ t''' : C)) ->
+    exists t''', (Γ ⊢< l > t' ⟹ t''' : A) /\ (Γ ⊢< l > t'' ⟹ t''' : A).
+Proof.
+  intros. destruct H1. destruct H1. destruct H1. destruct H1. destruct H1. exists x3. destruct H1.
+  destruct (ortho_validity _ _ _ _ _ H). destruct (ortho_validity _ _ _ _ _ H0).
+  destruct (ortho_validity _ _ _ _ _ H1). destruct (ortho_validity _ _ _ _ _ H2).
+  split.
+  - pose (K := type_unicity _ _ _ _ _ _ H7 H4). destruct K. eapply ortho_conv. rewrite <- H11. apply H1. rewrite H11 in H12. apply H12.
+  - pose (K := type_unicity _ _ _ _ _ _ H9 H6). destruct K. eapply ortho_conv. rewrite <- H11. apply H2. rewrite H11 in H12. apply H12.
+Qed.
 
 
 Fixpoint size (t : term) : nat := 
@@ -213,21 +324,164 @@ Qed.
 Theorem size_wk t ρ : size t = size (wk_tm ρ t).
 Proof.
   apply size_ren.
+Qed. 
+
+
+
+(* when applied to the ih, allows to also consider the more general case in which l can be prop.
+   this allows us to avoid doing a case analysis on l in the middle of the proof. *)
+Lemma ortho_diamond_helper2 u :
+  (forall t, size t < size u -> forall Γ i t' t'' A , Γ ⊢< ty i > t ⟹ t' : A -> 
+  Γ ⊢< ty i > t ⟹ t'' : A -> 
+  exists t''', (Γ ⊢< ty i > t' ⟹ t''' : A) /\ (Γ ⊢< ty i > t'' ⟹ t''' : A))
+  -> forall t, size t < size u -> forall Γ l t' t'' A,
+  Γ ⊢< l > t ⟹ t' : A -> 
+  Γ ⊢< l > t ⟹ t'' : A -> 
+  exists t''', (Γ ⊢< l > t' ⟹ t''' : A) /\ (Γ ⊢< l > t'' ⟹ t''' : A).
+Proof.
+  intros.
+  destruct l.
+  -  apply (H _ H0); auto.
+  - apply (ortho_diamond_prop _ _ _ _ _ H1 H2).
 Qed.
 
 
-Theorem ortho_diamond : 
-  forall Γ i t t' t'' A,
-    Γ ⊢< ty i > t ⟹ t' : A ->
-    Γ ⊢< ty i > t ⟹ t'' : A ->
-    exists t''', (Γ ⊢< ty i > t' ⟹ t''' : A) /\ (Γ ⊢< ty i > t'' ⟹ t''' : A).
-Proof.
-  intros Γ i. 
-  refine (@well_founded_ind _ (fun t u => size t > size u) _ _ _).
-  admit.
-  intros.
-  (* now we need an inversion principle for Γ ⊢< ty i > t ⟹ t' : A and  Γ ⊢< ty i > t ⟹ t'' : A 
-    which only requires us to consider compatible derivation rules, and which removes conversion *)
-Admitted.
 
+(* TODO: think of some nice tactics to make the easy cases of the proof more direct *)
+
+Theorem ortho_diamond : 
+  forall Γ i t t' t'' T,
+    Γ ⊢< ty i > t ⟹ t' : T ->
+    Γ ⊢< ty i > t ⟹ t'' : T ->
+    exists t''', (Γ ⊢< ty i > t' ⟹ t''' : T) /\ (Γ ⊢< ty i > t'' ⟹ t''' : T).
+Proof.
+  intros Γ i t. generalize t Γ i. clear Γ i t. 
+  
+  refine (@well_founded_ind _ (fun t u => size t < size u) _ _ _).
+  admit. intros.   
+
+  destruct x; eapply (ortho_diamond_helper _ _ _ _ _ _ H0 H1). 
+
+  (* var *)
+  - ttinv H0. ttinv H1.
+    destruct H0. destruct H0. rewrite H0. destruct H2. destruct H3. 
+    destruct H1. destruct H1. rewrite H1. destruct H5. destruct H6. 
+    eexists. eexists. eexists. eexists. exists (var n). split; apply ortho_var; eauto.
+  
+  (* sort *)
+    - ttinv H0. ttinv H1.
+    destruct H0. destruct H2. rewrite H2. destruct H3.
+    destruct H1. destruct H5. rewrite H5. destruct H6.
+    eexists. eexists. eexists. eexists. exists (Sort l). split; apply ortho_sort; eauto.
+
+
+  (* pi *)
+  - ttinv H0. ttinv H1. rename x1 into A. rename x2 into B. 
+    destruct H0 as (A' & H0). destruct H0 as (B' & H0). destruct H0. destruct H2. destruct H3. destruct H4. rewrite H0.
+    destruct H1 as (A'' & H1). destruct H1 as (B'' & H1). destruct H1. destruct H6.  destruct H7. destruct H8.  rewrite H1.
+
+    pose proof (H' := ortho_diamond_helper2 _ H). clear H.
+(* 
+
+    pose (IHt2' := ortho_diamond_helper2 _ IHt2). *)
+
+    epose proof (K1 := H' _ _ _ _ _ _ _ H3 H7). destruct K1 as (A''' & K1). destruct K1. shelve. Unshelve. simpl. lia.
+
+    epose proof (K2 := H' _ _ _ _ _ _ _ H4 H8). destruct K2 as (B''' & K2). destruct K2. shelve. Unshelve. simpl. lia.
+
+
+    assert (⊢ Γ). { pose (K := ortho_to_conv _ _ _ _ _ H3). apply validity_conv in K. destruct K. apply validity_ty in H13. destruct H13. auto. }
+
+    eexists. eexists. eexists. eexists. exists (Pi l l0 A''' B''').
+    split; apply ortho_pi; auto. 
+    + refine (ortho_conv_in_ctx _ _ _ _ _ _ _ H11). apply conv_ccons. apply refl_ctx. auto. auto using ortho_to_conv.
+    + refine (ortho_conv_in_ctx _ _ _ _ _ _ _ H12). apply conv_ccons. apply refl_ctx. auto. auto using ortho_to_conv.
+
+  (* lam *)
+  - admit.
+
+  (* app *)
+  - rename x1 into A. rename x2 into B. rename x3 into t. rename x4 into u. 
+    ttinv H0. clear H0. destruct h'. destruct H2.
+    ttinv H1. clear H1. destruct h'. destruct H4. 
+
+    rename t' into v'. rename t'' into v''.
+
+    destruct H3.
+    + destruct H5.
+      (* case app-cong x app-cong *)
+      ++ admit. 
+      (* case app-cong x beta *)
+      ++ destruct H3 as (A' & H3). destruct H3 as (B' & H3). destruct H3 as (t' & H3). destruct H3 as (u' & H3). 
+        destruct H3.  destruct H6.  destruct H7. destruct H8. 
+
+
+        rewrite H3. clear H3. clear v'.  
+
+        destruct H5 as (A2 & H5). destruct H5 as (B2 & H5). destruct H5 as (w & H5). destruct H5 as (w'' & H5). 
+        destruct H5 as (u'' & H5).  destruct H5.  destruct H5. destruct H10. destruct H11.  destruct H12. 
+        
+        rewrite H13. clear H13. clear v''. 
+
+        pose proof (H' := ortho_diamond_helper2 _ H). clear H.
+
+        rewrite H3 in *. clear H3. clear t.
+
+        epose proof (K1 := H' _ _ _ _ _ _ _ H9 H12). destruct K1 as (u''' & K1). destruct K1. shelve. Unshelve. simpl. lia. 
+        
+        rewrite <- H0 in *. clear H0 H1. clear l0.
+
+
+        assert (⊢ Γ) as H''. { pose (K := ortho_to_conv _ _ _ _ _ H3). apply validity_conv in K. destruct K. apply validity_ty in H0. destruct H0. auto. }
+
+        ttinv H8.
+        destruct h'. destruct H1. destruct H13. 
+        (* case lam-cong *)
+        * destruct H13 as (A2' & H13).  destruct H13 as (B2' & H13). destruct H13 as (w' & H13). 
+          destruct H13. destruct H14. destruct H15.  rewrite H13 in *. clear H13. clear t'.
+          clear H0.
+
+          assert (Γ,, (l, A) ⊢< ty i > w ⟹ w' : B). 
+          {
+            eapply ortho_conv_in_ctx in H16. shelve. apply conv_ccons. apply refl_ctx. auto. apply conv_sym. apply H5. 
+            Unshelve. apply (ortho_conv _ _ _ _ _ _ H16). apply conv_sym. auto. 
+          } 
+
+          epose proof (K1 := H' _ _ _ _ _ _ _ H0 H11). destruct K1 as (w''' & K1). destruct K1. shelve. Unshelve. simpl. lia. 
+
+          eexists. eexists. eexists. eexists.
+          exists (w''' <[ u''' ..]).
+          split.
+          (* closing left side *)
+          ** apply ortho_beta. 
+            *** eapply conv_trans. apply conv_sym. apply H6. eapply conv_trans. apply H5. apply H14. 
+            *** eapply conv_in_ctx_conv. apply conv_ccons. apply refl_ctx. auto. apply H6.
+                eapply conv_trans. apply conv_sym. apply H7. eapply conv_trans. apply H10. eapply conv_in_ctx_conv. 
+                apply conv_ccons. apply refl_ctx. auto. apply conv_sym. apply H5. auto.
+            *** eapply ortho_conv_in_ctx. apply conv_ccons. apply refl_ctx. auto. apply H6. eapply ortho_conv. apply H13. auto. 
+            *** eapply ortho_conv. apply H. auto.
+          (* closing right side *)
+          ** admit.
+          (* eapply ortho_subst_property. apply (well_scons _ _ _ (Γ,, (l, A))). shelve. simpl. apply H3.     *)
+        (* case eta *)
+        * admit.
+    
+    + destruct H5.
+      (* case beta x app-cong *)
+      ++ admit.
+      (* case beta x beta *)
+      ++ admit.
+  
+  (* Nat *)
+  - admit.
+  
+  (* zero *)
+  - admit.
+
+  (* succ *)
+  - admit.   
+  (* rec *)
+  - admit.   
+
+Admitted.
 
