theories/Inversion.v
@@ -1,0 +1,138 @@
+(** Inversion of typing *)
+
+From Stdlib Require Import Utf8 String List Arith Lia.
+From TypedConfluence.autosubst Require Import unscoped AST SubstNotations RAsimpl
+  AST_rasimpl.
+From TypedConfluence Require Import Util BasicAST Contexts Typing Confluence.
+From Stdlib Require Import Setoid Morphisms Relation_Definitions.
+
+From Equations Require Import Equations.
+
+Import ListNotations.
+Import CombineNotations.
+
+Set Default Goal Selector "!".
+(* 
+Derive NoConfusion NoConfusionHom for list.
+Derive NoConfusion NoConfusionHom for term.
+Derive Signature for typing.
+
+Require Import Equations.Prop.DepElim.
+
+Ltac destruct_exists h :=
+  match type of h with
+  | ∃ _, _ => destruct h as [? h] ; destruct_exists h
+  | _ => idtac
+  end.
+
+Ltac destruct_all_exists :=
+  repeat
+  match goal with
+  | h : ∃ _, _ |- _ => destruct h
+  end.
+
+#[local] Ltac do_eexists :=
+  lazymatch goal with
+  | |- ∃ _, _ => eexists
+  end.
+
+#[local] Ltac invtac h :=
+  pose (H := proj2 (validity_ty _ _ _ _ h)) ; generalize H ; clear H ; dependent induction h ; [
+    intros H' ; repeat do_eexists ; intuition eauto ; apply (refl_ty _ _ _ _ H')
+  | intros H' ; destruct_all_exists ; repeat do_eexists ; intuition eauto ;
+    eapply conv_trans ; eauto
+  ]. *)
+
+Lemma type_var_inv Γ l x t A :
+  Γ ⊢< l > var x ⟹ t : A →
+  ∃ B,
+    t = var x  ∧
+    nth_error Γ x = Some (l, B) ∧
+    Γ ⊢< Ax l > (plus (S x)) ⋅ B ≡ A : Sort l.
+Proof.
+  (* pose (H := proj2 (validity_ty _ _ _ _ h)).
+  generalize H. clear H.
+  dependent induction h.
+  - intro H'. repeat do_eexists . intuition eauto .  apply (refl_ty _ _ _ _ H').
+  - intro H'. pose (IHh' := IHh H').  destruct_all_exists. repeat do_eexists . intuition eauto . eapply conv_trans.
+  eexists. split. 
+    + shelve. + apply (refl_ty _ _ _ _ H1). Unshelve. auto.
+  
+  invtac h. *)
+Admitted.
+
+Lemma type_sort_inv Γ l l' t A :
+  Γ ⊢< l' > Sort l ⟹ t : A →
+  t = Sort l  ∧ l' = Ax (Ax l)  ∧
+  Γ ⊢< Ax (Ax (Ax l)) > Sort (Ax l) ≡ A : Sort (Ax l).
+Proof.
+Admitted.
+(* 
+Lemma type_pi_inv Σ Ξ Γ A B T :
+  Σ ;; Ξ | Γ ⊢ Pi A B : T →
+  ∃ i j,
+    Σ ;; Ξ | Γ ⊢ A : Sort i ∧
+    Σ ;; Ξ | Γ ,, A ⊢ B : Sort j ∧
+    Σ ;; Ξ ⊢ Sort (max i j) ≡ T.
+Proof.
+  intros h. invtac h.
+Qed.
+
+Lemma type_lam_inv Σ Ξ Γ A t T :
+  Σ ;; Ξ | Γ ⊢ lam A t : T →
+  ∃ i j B,
+    Σ ;; Ξ | Γ ⊢ A : Sort i ∧
+    Σ ;; Ξ | Γ ,, A ⊢ B : Sort j ∧
+    Σ ;; Ξ | Γ ,, A ⊢ t : B ∧
+    Σ ;; Ξ ⊢ Pi A B ≡ T.
+Proof.
+  intros h. invtac h.
+Qed.
+
+Lemma type_app_inv Σ Ξ Γ u v T :
+  Σ ;; Ξ | Γ ⊢ app u v : T →
+  ∃ i j A B,
+    Σ ;; Ξ | Γ ⊢ u : Pi A B ∧
+    Σ ;; Ξ | Γ ⊢ v : A ∧
+    Σ ;; Ξ | Γ ⊢ A : Sort i ∧
+    Σ ;; Ξ | Γ ,, A ⊢ B : Sort j ∧
+    Σ ;; Ξ ⊢ B <[ v .. ] ≡ T.
+Proof.
+  intros h. invtac h.
+Qed.
+
+Lemma type_const_inv Σ Ξ Γ c ξ T :
+  Σ ;; Ξ | Γ ⊢ const c ξ : T →
+  ∃ Ξ' A t,
+    Σ c = Some (Def Ξ' A t) ∧
+    inst_typing Σ Ξ Γ ξ Ξ' ∧
+    closed A = true ∧
+    Σ ;; Ξ ⊢ inst ξ A ≡ T.
+Proof.
+  intros h. invtac h.
+Qed.
+
+Lemma type_assm_inv Σ Ξ Γ x T :
+  Σ ;; Ξ | Γ ⊢ assm x : T →
+  ∃ A,
+    ictx_get Ξ x = Some (Assm A) ∧
+    closed A = true ∧
+    Σ ;; Ξ ⊢ A ≡ T.
+Proof.
+  intros h. invtac h.
+Qed. *)
+
+Ltac ttinv h h' :=
+  lazymatch type of h with
+  _ ⊢< _ > ?t : _ =>
+    lazymatch t with
+    | var _ => eapply type_var_inv in h as h'
+    | Sort _ => eapply type_sort_inv in h as h'
+    | _ => h'
+    (* | Pi _ _ => eapply type_pi_inv in h as h'
+    | lam _ _ => eapply type_lam_inv in h as h'
+    | app _ _ => eapply type_app_inv in h as h'
+    | const _ _ => eapply type_const_inv in h as h'
+    | assm _ => eapply type_assm_inv in h as h' *)
+    end
+  end.
